ifexpr validate commutes in own folder

Validator/Regex/Enter.lean
@@ -1,19 +1,11 @@
 import Validator.Std.Vec
 
 import Validator.Regex.Extract
-import Validator.Regex.IfExpr.IfExpr
 import Validator.Regex.Num
 import Validator.Regex.Regex
 
 namespace Regex
 
-def enter (r: Regex σ): IfExpr σ (symbols r) := IfExpr.mk (extract r).2
+def enter (r: Regex σ) := (extract r).2
 
-def enter_with_alloc (r: Regex σ) := (extract r).2
-
-namespace IfExpr
-
-#guard enter (Regex.or (Regex.symbol 'a') (Regex.symbol 'b')) =
-  IfExpr.expr 'a'
-    (IfExpr.expr 'b' (IfExpr.res  #v[true, true]) (IfExpr.res  #v[true, false]))
-    (IfExpr.expr 'b' (IfExpr.res  #v[false, true]) (IfExpr.res  #v[false, false]))
+#guard enter (Regex.or (Regex.symbol 'a') (Regex.symbol 'b')) = #v['a','b']
