Validator/Regex/Room.lean
@@ -11,25 +11,14 @@ import Validator.Regex.Regex
 -- room, since we enter and leave
 -- Also this a power in One Piece, which seems appropriate: https://onepiece.fandom.com/wiki/Ope_Ope_no_Mi
 def Regex.Room.derive (Φ: σ → Bool) (r: Regex σ): Regex σ :=
-  enter r |> IfExpr.eval Φ |> leave r
-
-def Regex.Room.derive_with_alloc (Φ: σ → Bool) (r: Regex σ): Regex σ :=
-  enter_with_alloc r |> Vector.map Φ |> leave r
+  enter r |> Vector.map Φ |> leave r
 
 def Regex.Room.validate (Φ: σ → α → Bool) (r: Regex σ) (xs: List α): Bool :=
   null (List.foldl (fun dr x => Regex.Room.derive (flip Φ x) dr) r xs)
 
-lemma Regex.Room.derive_is_Regex.Room.derive_with_alloc (Φ: σ → Bool) (r: Regex σ):
-  Regex.Room.derive Φ r = Regex.Room.derive_with_alloc Φ r := by
-  unfold Regex.Room.derive_with_alloc
-  unfold Regex.Room.derive
-  unfold Regex.enter
-  unfold Regex.enter_with_alloc
-  rw [IfExpr.eval_is_map]
-
 lemma Regex.Room.derive_is_Regex_derive (Φ: σ → α → Bool) (r: Regex σ) (a: α):
   Regex.Room.derive (flip Φ a) r = Regex.derive Φ r a := by
-  simp only [Room.derive, enter, leave, <- Vector.map_zip_is_zip_map, flip, IfExpr.eval_is_map]
+  simp only [Room.derive, enter, leave, <- Vector.map_zip_is_zip_map, flip]
   rw [<- Regex.extract_replace_is_map]
   rw [Regex.Point.regex_derive_is_point_derive]
 
