Validator/Regex/IfExpr/Enter.lean
@@ -1,0 +1,15 @@
+import Validator.Std.Vec
+
+import Validator.Regex.Extract
+import Validator.Regex.IfExpr.IfExpr
+import Validator.Regex.Num
+import Validator.Regex.Regex
+
+namespace Regex.IfExpr
+
+def enter (r: Regex σ): IfExpr σ (symbols r) := IfExpr.mk (extract r).2
+
+#guard enter (Regex.or (Regex.symbol 'a') (Regex.symbol 'b')) =
+  IfExpr.expr 'a'
+    (IfExpr.expr 'b' (IfExpr.res  #v[true, true]) (IfExpr.res  #v[true, false]))
+    (IfExpr.expr 'b' (IfExpr.res  #v[false, true]) (IfExpr.res  #v[false, false]))
